Added tactics for soundness proofs (they are still somewhat stuck in ProdView.v)

theories/Views/ProdView.v
@@ -1,3 +1,6 @@
+Add Rec LoadPath "/Users/jebe/git/coq-ext-lib/theories" as ExtLib.
+Add Rec LoadPath "/Users/jebe/git/mirror-core/theories" as MirrorCore.
+
 Require Import ExtLib.Core.RelDec.
 Require Import ExtLib.Data.Fun.
 Require Import ExtLib.Data.Map.FMapPositive.
@@ -5,6 +8,7 @@ Require Import ExtLib.Data.SumN.
 Require Import ExtLib.Data.Positive.
 Require Import ExtLib.Tactics.Consider.
 Require Import ExtLib.Tactics.
+Require Import ExtLib.Relations.TransitiveClosure.
 
 Require Import MirrorCore.TypesI.
 Require Import MirrorCore.syms.SymEnv.
@@ -13,7 +17,6 @@ Require Import MirrorCore.Lambda.Expr.
 Require Import MirrorCore.Lambda.Ptrns.
 Require Import MirrorCore.Views.Ptrns.
 Require Import MirrorCore.Views.FuncView.
-Require Import MirrorCore.Views.TrmD.
 Require Import MirrorCore.RTac.Simplify.
 Require Import MirrorCore.Lambda.AppN.
 Require Import MirrorCore.Lambda.RedAll.
@@ -30,7 +33,7 @@ Inductive prod_func {typ : Type} :=
 Implicit Arguments prod_func [].
 
 Section ProdFuncInst.
-  Context {typ func : Type} {HR : RType typ}.
+  Context {typ func : Type} {RType_typ : RType typ}.
   Context {RelDec_typ : RelDec (@eq typ)}.
   Context {RelDecCorrect_typ : RelDec_Correct RelDec_typ}.
   
@@ -58,53 +61,50 @@ Section ProdFuncInst.
       | _, _ => None
     end.
 
-  Definition prodE {A B : Type} {t u : typ} (e1 : typD t = A) (e2 : typD u = B) : 
-    typD (tyProd t u) = (A * B)%type :=
-    eq_ind (typD t) (fun X : Type => typD (tyProd t u) = (X * B)%type)
-      (eq_ind (typD u) (fun Y : Type => typD (tyProd t u) = (typD t * Y)%type)
-              (typ2_cast t u) B e2) A e1.  
-  
-  Definition prodD t u (p : typD (tyProd t u)) : typD t * typD u :=
-    trmD p (prodE (t := t) (u := u) eq_refl eq_refl).
-  
-  Definition prodR t u (p : typD t * typD u) : typD (tyProd t u) :=
-    trmR p (prodE (t := t) (u := u) eq_refl eq_refl).
-  
-  Lemma prodDR (t u : typ) A B C D (x : A) (y : B) (e1 : typD t = A) 
-        (e2 : typD u = B) (e3 : typD t = C) (e4 : typD u = D) :
-    trmD (trmR (x, y) (prodE e1 e2)) (prodE e3 e4) = 
-    (trmD (trmR x e1) e3, trmD (trmR y e2) e4).
-  Proof.
-    unfold trmD, trmR, prodE, eq_ind, eq_rect_r, eq_rect, eq_sym, id.
-    clear.
-    revert e1 e2 e3 e4.
-    generalize (typ2_cast t u).
-    unfold tyProd.
-    generalize dependent (typ2 t u).
-    generalize dependent (typD t).
-    generalize dependent (typD u).
-    do 3 intros.
-    generalize dependent (typD t0).
-    intros; repeat subst. reflexivity.
-  Qed.
+  Definition castD F U {T : Typ0 _ U} (val : F (typD (typ0 (F:=U)))) : F U :=
+    match @typ0_cast typ _ _ T in _ = x return F x with
+      | eq_refl => val
+    end.
 
-  Definition pairD (t u : typ) : typD (tyArr t (tyArr u (tyProd t u))) :=
-    tyArrR2 (fun a b => prodR t u (a, b)).
+  Definition castR F U {T : Typ0 _ U} (val : F U) : F (typD (typ0 (F:=U))) :=
+    match eq_sym (@typ0_cast typ _ _ T) in _ = x return F x with
+    | eq_refl => val
+    end.
 
-  Definition fstD (t u : typ) : typD (tyArr (tyProd t u) t) :=
-    tyArrR (fun p => fst (prodD t u p)).
+  Existing Instance Typ2_App.
+  Existing Instance Typ1_App.
+  Existing Instance Typ0_term.
+
+  Implicit Arguments castD [[T]].
+  Implicit Arguments castR [[T]].
+
+  Definition pairD t u : typD (tyArr t (tyArr u (tyProd t u))) -> 
+                         Fun (typD t) (Fun (typD u) (typD t * typD u)) :=
+    castD id (Fun (typD t) (Fun (typD u) (typD t * typD u)%type)).
+
+  Definition pairR t u : typD (tyArr t (tyArr u (tyProd t u))) :=
+    castR id (Fun (typD t) (Fun (typD u) (typD t * typD u))) pair.
+
+  Definition fstD t u : typD (tyArr (tyProd t u) t) -> Fun (typD t * typD u) (typD t) :=
+    castD id (Fun (typD t * typD u) (typD t)).
+
+  Definition fstR t u : typD (tyArr (tyProd t u) t) :=
+    castR id (Fun (typD t * typD u) (typD t)) fst.
+
+  Definition sndD t u : typD (tyArr (tyProd t u) u) -> Fun (typD t * typD u) (typD u) :=
+    castD id (Fun (typD t * typD u) (typD u)).
   
-  Definition sndD (t u : typ) : typD (tyArr (tyProd t u) u) :=
-    tyArrR (fun p => snd (prodD t u p)).
+  Definition sndR t u : typD (tyArr (tyProd t u) u) :=
+    castR id (Fun (typD t * typD u) (typD u)) snd.
   
   Definition prod_func_symD bf :=
     match bf as bf return match typeof_prod_func bf return Type with
 			    | Some t => typD t
 			    | None => unit
 			  end with
-      | pPair t u => pairD t u
-      | pFst t u => fstD t u
-      | pSnd t u => sndD t u
+      | pPair t u => pairR t u
+      | pFst t u => fstR t u
+      | pSnd t u => sndR t u
     end.
 
   Global Instance RSym_ProdFunc
@@ -129,10 +129,16 @@ Section ProdFuncInst.
   
 End ProdFuncInst.
 
+Implicit Arguments castD [[RType_typ] [T]].
+Implicit Arguments castR [[RType_typ] [T]].
+
 Section MakeProd.
   Context {typ func : Type} {RType_typ : RType typ}.
   Context {HF : FuncView func (prod_func typ)}.
-  
+  Context {RelDec_typ : RelDec (@eq typ)}.
+  Context {Typ2_tyArr : Typ2 _ Fun}.
+  Context {Typ2_tyProd : Typ2 _ prod}.
+
   Definition fPair t u := f_insert (pPair t u).
   Definition fFst t u := f_insert (pFst t u).
   Definition fSnd t u := f_insert (pSnd t u).
@@ -140,40 +146,111 @@ Section MakeProd.
   Definition mkPair (t u : typ) (a b : expr typ func) := App (App (Inj (fPair t u)) a) b.
   Definition mkFst (t u : typ) (p : expr typ func) := App (Inj (fFst t u)) p.
   Definition mkSnd (t u : typ) (p : expr typ func) := App (Inj (fSnd t u)) p.
+  Print ptrn_view.
 
-  Definition fptrnPair : ptrn func unit :=
-    fun f _ good bad => 
-    match f_view f with
-      | Some (pPair _ _) => good tt
-      | _ => bad f
-    end.
+  Definition fptrnPair {T : Type} (p : Ptrns.ptrn (typ * typ) T) : ptrn (prod_func typ) T :=
+    fun f U good bad =>
+      match f with 
+        | pPair t u => p (t, u) U good (fun x => bad f)
+        | _ => bad f
+      end.
 
-  Definition ptrnPair {A B : Type} 
+  Definition fptrnFst {T : Type} (p : Ptrns.ptrn (typ * typ) T) : ptrn (prod_func typ) T :=
+    fun f U good bad =>
+      match f with 
+        | pFst t u => p (t, u) U good (fun x => bad f)
+        | _ => bad f
+      end.
+
+  Definition fptrnSnd {T : Type} (p : Ptrns.ptrn (typ * typ) T) : ptrn (prod_func typ) T :=
+    fun f U good bad =>
+      match f with 
+        | pSnd t u => p (t, u) U good (fun x => bad f)
+        | _ => bad f
+      end.
+
+  Global Instance fptrnPair_ok {T : Type} {p : ptrn (typ * typ) T} {Hok : ptrn_ok p} : 
+    ptrn_ok (fptrnPair p).
+  Proof.
+    red; intros.
+    destruct x; simpl; [destruct (Hok (t, t0))| |].
+    { left. destruct H; exists x. revert H. compute; intros.
+      rewrite H. reflexivity. }
+    { right; unfold Fails in *; intros; simpl; rewrite H; reflexivity. }
+    { right; unfold Fails; reflexivity. }
+    { right; unfold Fails; reflexivity. }
+  Qed.
+     
+  Global Instance fptrnFst_ok {T : Type} {p : ptrn (typ * typ) T} {Hok : ptrn_ok p} : 
+    ptrn_ok (fptrnFst p).
+  Proof.
+    red; intros.
+    destruct x; simpl; [|destruct (Hok (t, t0)) |].
+    { right; unfold Fails; reflexivity. }
+    { left. destruct H; exists x. revert H. compute; intros.
+      rewrite H. reflexivity. }
+    { right; unfold Fails in *; intros; simpl; rewrite H; reflexivity. }
+    { right; unfold Fails; reflexivity. }
+  Qed.
+     
+  Global Instance fptrnSnd_ok {T : Type} {p : ptrn (typ * typ) T} {Hok : ptrn_ok p} : 
+    ptrn_ok (fptrnSnd p).
+  Proof.
+    red; intros.
+    destruct x; simpl; [| |destruct (Hok (t, t0))].
+    { right; unfold Fails; reflexivity. }
+    { right; unfold Fails; reflexivity. }
+    { left. destruct H; exists x. revert H. compute; intros.
+      rewrite H. reflexivity. }
+    { right; unfold Fails in *; intros; simpl; rewrite H; reflexivity. }
+  Qed.
+     
+  Definition ptrnPair {A B T : Type} 
+             (p : ptrn (typ * typ) T)
              (a : ptrn (expr typ func) A)
              (b : ptrn (expr typ func) B) : ptrn (expr typ func) (A * B) :=
-    pmap (fun x => match x with | (_, a, b) => (a, b) end) (app (app (inj fptrnPair) a) b).
+    pmap (fun x => match x with | (_, a, b) => (a, b) end) 
+         (app (app (inj (ptrn_view _ (fptrnPair p))) a) b).
 
-  Definition fptrnFst : ptrn func unit :=
-    fun f _ good bad => 
-    match f_view f with
-      | Some (pFst _ _) => good tt
-      | _ => bad f
-    end.
+  Definition ptrnFst {A T : Type} 
+             (p : ptrn (typ * typ) T)
+             (a : ptrn (expr typ func) A) : ptrn (expr typ func) A :=
+    pmap snd (app (inj (ptrn_view _ (fptrnFst p))) a).
 
-  Definition ptrnFst {A : Type} 
-             (p : ptrn (expr typ func) A) : ptrn (expr typ func) A :=
-    pmap snd (app (inj fptrnFst) p).
-
-  Definition fptrnSnd : ptrn func unit :=
-    fun f _ good bad => 
-    match f_view f with
-      | Some (pSnd _ _) => good tt
-      | _ => bad f
-    end.
-
-  Definition ptrnSnd {A : Type} 
-             (p : ptrn (expr typ func) A) : ptrn (expr typ func) A :=
-    pmap snd (app (inj fptrnSnd) p).
+  Definition ptrnSnd {A T : Type} 
+             (p : ptrn (typ * typ) T)
+             (a : ptrn (expr typ func) A) : ptrn (expr typ func) A :=
+    pmap snd (app (inj (ptrn_view _ (fptrnSnd p))) a).
+  
+  Lemma Succeeds_fptrnPair {T : Type} (f : prod_func typ) (p : ptrn (typ * typ) T) res 
+        (H : Succeeds f (fptrnPair p) res) :
+    exists t u, f = pPair t u.
+  Proof.
+    unfold Succeeds, fptrnPair in H.
+    specialize (H bool (fun _ => true) (fun _ => false)).
+    destruct f; try congruence.
+    exists t, t0; reflexivity.
+  Qed.
+  
+  Lemma Succeeds_fptrnFst  {T : Type} (f : prod_func typ) (p : ptrn (typ * typ) T) res 
+        (H : Succeeds f (fptrnFst p) res) :
+    exists t u, f = pFst t u.
+  Proof.
+    unfold Succeeds, fptrnFst in H.
+    specialize (H bool (fun _ => true) (fun _ => false)).
+    destruct f; try congruence.
+    exists t, t0; reflexivity.
+  Qed.
+  
+  Lemma Succeeds_fptrnSnd  {T : Type} (f : prod_func typ) (p : ptrn (typ * typ) T) res 
+        (H : Succeeds f (fptrnSnd p) res) :
+    exists t u, f = pSnd t u.
+  Proof.
+    unfold Succeeds, fptrnSnd in H.
+    specialize (H bool (fun _ => true) (fun _ => false)).
+    destruct f; try congruence.
+    exists t, t0; reflexivity.
+  Qed.
   
 End MakeProd.
 
@@ -181,18 +258,26 @@ Section Tactics.
   Context {typ func : Type}.
   Context {FV : FuncView func (prod_func typ)}.
   Context {RType_typ : RType typ} {RSym_func : RSym func}.
+  Context {RTypeOk_typ : @RTypeOk _ RType_typ}.
+  Context {RSymOk_func : RSymOk RSym_func}.
   Context {Typ2_tyArr : Typ2 _ Fun}.
+  Context {Typ2_tyProd : Typ2 _ prod}.
+  Context {Typ2Ok_tyArr : Typ2Ok Typ2_tyArr}.
+  Context {Typ2Ok_tyProd : Typ2Ok Typ2_tyProd}.
+  Context {RelDecEq : RelDec (@eq typ)}.
+  Context {RelDecCorrectEq : RelDec_Correct RelDecEq}.
+  Context {FVOk : FuncViewOk (typ := typ) FV RSym_func RSym_ProdFunc}.
+
+  Let tyArr := @typ2 _ _ _ Typ2_tyArr.
+  Let tyProd := @typ2 _ _ _ Typ2_tyProd.
   
   Definition red_fst_ptrn : ptrn (expr typ func) (expr typ func) :=
-    pmap (fun xy => fst xy) (ptrnFst (ptrnPair get ignore)).
-
-  Definition pdefault_id {X} (p : ptrn X X) : tptrn X X :=
-    fun e => pdefault p e e. 
+    pmap (fun xy => fst xy) (ptrnFst ignore (ptrnPair ignore get ignore)).
 
   Definition red_fst := run_tptrn (pdefault_id red_fst_ptrn).
 
   Definition red_snd_ptrn : ptrn (expr typ func) (expr typ func) :=
-    pmap (fun xy => snd xy) (ptrnSnd (ptrnPair ignore get)).
+    pmap (fun xy => snd xy) (ptrnSnd ignore (ptrnPair ignore ignore get)).
 
   Definition red_snd := run_tptrn (pdefault_id red_snd_ptrn).
 
@@ -200,53 +285,108 @@ Section Tactics.
                              (fun _ _ _ _ => 
                                 (beta_all (fun _ e args => red_fst (apps e args)))).
 
-  Lemma run_tptrn_id_sound tus tvs t p e val
-        (H : ExprDsimul.ExprDenote.exprD' tus tvs t e = Some val)
-        (HSucceeds : forall e', Succeeds e p e' ->
-                                ExprDsimul.ExprDenote.exprD' tus tvs t e' = Some val) :
-    ExprDsimul.ExprDenote.exprD' tus tvs t
-                                 (run_tptrn (pdefault_id p) e) = Some val.
+  Ltac destruct_prod :=
+    match goal with 
+      | p : ?A * ?B |- _ => destruct p; destruct_prod
+      | _ => idtac
+    end.
+
+  Existing Instance Typ2_App.
+  Existing Instance Typ1_App.
+  Existing Instance Typ0_term.
+  Existing Instance MirrorCore.ExprI.Applicative_exprT.
+
+Require Import MirrorCore.Util.Compat.
+
+Theorem exprT_App_Fun tus tvs T U (T0 : Typ0 _ T) (U0 : Typ0 _ U)
+        (e1 : exprT tus tvs (Fun T U))
+        (e2 : exprT tus tvs T) :
+@exprT_App typ _ Typ2_tyArr tus tvs (@typ0 _ _ T _) (@typ0 _ _ U _) (@castR typ _ (exprT tus tvs) _ _ e1)
+                 (@castR typ _ (exprT tus tvs) _ _ e2) =
+      @castR typ _ (exprT tus tvs) U U0 (Applicative.ap e1 e2).
   Proof.
+    unfold exprT_App. simpl. intros.
+    unfold castR. simpl.
+    generalize dependent (typ2_cast (typ0 (F:=T)) (typ0 (F:=U))).
+    generalize dependent (typ0_cast (F:=T)).
+    generalize dependent (typ0_cast (F:=U)).
+    intros.
+    autorewrite_with_eq_rw.
+    generalize dependent (typD (typ2 (typ0 (F:=T)) (typ0 (F:=U)))).
+    intros. subst T1.
+    admit.
+(*
+    destruct (eq_sym e0).
+    destruct (eq_sym e). simpl. reflexivity.*)
+  Admitted.
+
+Theorem exprT_App_Fun' tus tvs T U (T0 : Typ0 _ T) (U0 : Typ0 _ U)  P
+        (e1 : exprT tus tvs (Fun T U))
+        (e2 : exprT tus tvs T) 
+        (Hres : P (@castR typ _ (exprT tus tvs) U U0 (Applicative.ap e1 e2))) :
+  P (@exprT_App typ _ Typ2_tyArr tus tvs (@typ0 _ _ T _) (@typ0 _ _ U _) (@castR typ _ (exprT tus tvs) _ _ e1) (@castR typ _ (exprT tus tvs) _ _ e2)).
+  Proof.
+    subst. rewrite exprT_App_Fun. assumption.
+  Qed.
+
+  Lemma exprT_App_castR_pure {A : Type} {T0 : Typ0 RType_typ A} tus tvs (f : exprT tus tvs A) :
+    (fun us vs => castR typ id A (f us vs)) = 
+    (castR typ (exprT tus tvs) A f).
+  Proof.
+    unfold castR, eq_sym; simpl.
+    Require Import FunctionalExtensionality.
+    do 2 (apply functional_extensionality; intros).
     admit.
   Admitted.
+
+
+    Ltac force_apply lem :=
+      let L := fresh "L" in 
+      pose proof lem as L; apply L; clear L.
+
+Ltac ptrn_prod_sound_step :=
+  match goal with
+    | H : Succeeds _ (fptrnPair _) _ |- _ => 
+      apply Succeeds_fptrnPair in H; destruct H as [? [? ?]]; repeat subst
+    | H : Succeeds _ (fptrnFst _) _ |- _ => 
+      apply Succeeds_fptrnFst in H; destruct H as [? [? ?]]; repeat subst
+    | H : Succeeds _ (fptrnSnd _) _ |- _ => 
+      apply Succeeds_fptrnSnd in H; destruct H as [? [? ?]]; repeat subst
+end.
+
+Ltac ptrn_sound_step :=
+  first [
+      ptrn_base_sound_step |
+      ptrn_prod_sound_step
+    ].
+
+Ltac exprT_App_red :=
+    match goal with
+      | |- context [castR _ id _ _] => rewrite exprT_App_castR_pure
+      | |- context [@exprT_App _ _ _ ?tus ?tvs _ _ (castR _ _ (Fun ?t1 ?t2) _) ?v] =>
+
+        first [
+            force_apply (@exprT_App_Fun' tus tvs t1 t2 _ _) |
+            replace v with (castR typ (exprT tus tvs) _ v) by reflexivity;
+              force_apply (@exprT_App_Fun' tus tvs t1 t2 _ _)
+          ]
+    end. 
+
 
   Lemma red_fst_ok : partial_reducer_ok (fun e args => red_fst (apps e args)).
   Proof.
     unfold partial_reducer_ok; intros.
     exists val; split; [|reflexivity].
-    generalize dependent (apps e es). clear e es; intros e H.
+    generalize dependent (apps e es); clear e es; intros e H.
     unfold red_fst.
-
-    apply run_tptrn_id_sound; [assumption|].
-    intros.
-    unfold red_fst_ptrn in H0.
-    apply Succeeds_pmap in H0.
-    destruct H0 as [[x y] [H1 H2]].
-    simpl in H2; subst.
-    unfold ptrnFst in H1.
-    apply Succeeds_pmap in H1. 
-    destruct H1 as [[x' [y' z']] [H1 H2]].
-    simpl in H2. inversion H2; subst. clear H2.
-    apply Succeeds_app in H1.
-    destruct H1 as [l [r [Heq [H1 H2]]]]. subst. simpl in H1, H2.
-    apply Succeeds_inj in H1.
-    destruct H1 as [f [Heq H1]].
-    subst.
-    unfold ptrnPair in H2.
-    apply Succeeds_pmap in H2.
-    destruct H2 as [[[x y] z] [H2 H3]].
-    inversion H3; subst. clear H3.
-    apply Succeeds_app in H2.
-    destruct H2 as [l' [r' [Heq [H2 H3]]]].
-    subst.
-    apply Succeeds_app in H2.
-    destruct H2 as [l'' [r'' [Heq [H2 H4]]]].
-    simpl in *.
-    apply Succeeds_inj in H2.
-    subst.
-    destruct H2 as [f' [Heq H2]].
-    apply Succeeds_get in H4. subst.
-
-    Admitted.
+    
+    apply run_tptrn_id_sound; [assumption|]; intros.
+    unfold red_fst_ptrn, ptrnFst, ptrnPair in H0.
+    repeat ptrn_sound_step.
+    destruct_prod.
+    unfold pairR, fstR.
+    repeat exprT_App_red.
+    apply H6.
+  Qed.
 
 End Tactics.
